#+TITLE: Assignment 1
#+AUTHOR: Jan Hendron(s1049777)
#+OPTIONS: toc:nil
#+LATEX_HEADER:

* Exercise 6
We must make some case distinctions in this question

1. We assume that \(a = 0, b = 0\)

   Then we just have that \(y=x\)

2. We assume that \(a < 0, b = 0\)

   Then we have
   \begin{gather*}
   y = a + (0 - a)x \\
    y = a-ax \\
    y = x
   \end{gather*}

   So again \(y = x\)

3. We assume that \(a = 0, b < 0\)

   Then we get
   \begin{gather*}
   y = 0 + (b - 0)x \\
   y = bx \\
   \end{gather*}

4. We assume that \(a = 0, b > 0\)

* Exercise 7
To prove that a function is odd, we must show that \(-f(x)=f(-x)\; \forall x\in D\), and to prove that a function is even, we must show that \(f(x) = f(-x)\; \forall x \in D\)

a.
   \begin{align*}
   \textrm{\(f(-x)\) should be equal to this if it is even}\\
   f(x) &= 3x-x^{3} \\
   & \\
   \textrm{\(f(-x)\) should be equal to this if it is odd} \\
   -f(x) &= -(3x-x^{3})\\
   &= -3x+x^{3} \\
   &= x^{3}-3x \\
   &  \\
   \textrm{Here we test if either it true} \\
   f(-x) &= 3(-x)-(-x)^{3}   \\
   &= -3x-(-x^3) \\
   &= -3x+x^3 \\
   &= x^3-3x
   \end{align*}
   Therefore, \(f(x) = 3x-x^{3}\) is an *odd* function
b.
   \begin{align*}
   \textrm{\(f(-x)\) should be equal to this if it is even} \\
    f(x) &= \sqrt[3]{(1-x)^{2}} + \sqrt[3]{(1+x)^2} \\
    \textrm{\(f(-x)\) should be equal to this if it is odd} \\
    -f(x) &= -\left(\sqrt[3]{(1-x)^2} + \sqrt[3]{(1+x)^2}\right)\\
    &= - \sqrt[3]{(1-x)^2} - \sqrt[3]{(1+x)^2}\\
    \textrm{Here we test if either are true}\\
    f(-x) &= \sqrt[3]{(1-(-x))^{2}} + \sqrt[3]{(1+(-x))^2} \\
    &= \sqrt[3]{(1+x)^{2}} + \sqrt[3]{(1-x)^2} \\
    &\textrm{Rearrange} \\
    &= \sqrt[3]{(1-x)^{2}} + \sqrt[3]{(1+x)^2} \\
   \end{align*}
   Therefore, \(f(x) = \sqrt[3]{(1-x)^{2}} + \sqrt[3]{(1+x)^2} \) is an *even* function
* Exercise 8
* Exercise 9
1. In order to compute the inverse of a function \(f^{-1}(x)\), you have to express the function in terms of \(x\), and then change the variables, so from the function \(y = \frac{ax+b}{cx+d}\)

         \begin{gather*}
         y = \frac{ax+b}{cx+d} \\
         y(cx+d) = ax+b \\
         cxy + dy = ax+b \\
         cxy - ax =b-dy \\
         x(cy-a) = b-dy \\
         x = \frac{b-dy}{cy-a}\\
         y = \frac{b-dx}{cx-a}
         \end{gather*}

2.
* Exercise 10
a)
\begin{gather*}
\lim_{x\to2} \frac{x-2}{x^{2}+x-6} \\
\end{gather*}
This will be done using the *simplify* method
Factorize the denominator
\begin{gather*}
\frac{x-2}{(x-2)(x+3)}
\end{gather*}
Cancel the \((x-2)\) on both sides of the fraction
\begin{gather*}
\frac{1}{x+3} \\
\frac{1}{2+3} \\
\lim_{x\to2} \frac{x-2}{x^{2}+x-6} = \frac{1}{5} \\
\end{gather*}
b)
c)
d)
